\documentclass{lehramt-informatik-aufgabe}
\liLadePakete{formale-sprachen}
\begin{document}
\liAufgabenTitel{Chomsky-Normalform}
\section{Chomsky-Normalform
\index{Chomsky-Normalform}
\footcite{theo:ab:2}}

Überführen Sie jeweils die angegebene kontextfreie Grammatik in
Chomsky-Normalform.

\begin{enumerate}
\item $G = (\{a, b, c\}, \{S, A, B, C, X\}, P, S)$ mit $P$:

\begin{liProduktionsRegeln}
S -> XAB | epsilon,
A -> aAB | AB | c,
B -> BB | C | a,
C -> CC | c | epsilon,
X -> A | b
\end{liProduktionsRegeln}

\item $G = (\{a, b, c\}, \{S, T\}, P, S)$ mit $P$:

\begin{liProduktionsRegeln}
S -> aSbS | T,
T -> cT | c
\end{liProduktionsRegeln}

\item $G = (\{a, b, c\}, \{S, A, B\}, P, S)$ mit $P$:

\begin{liProduktionsRegeln}
S -> AB,
A -> aAA | epsilon,
B -> bBB | epsilon
\end{liProduktionsRegeln}
\end{enumerate}

\end{document}
